DataflowRewriter/Examples/NoC/2x2.lean
@@ -18,7 +18,13 @@ abbrev Data := ℕ
 abbrev FlitHeader := Nat -- TODO: Dest RouterID
 abbrev RouterID := Nat -- TODO: a Fin probably
 abbrev netsz := 4
-abbrev Direction := Nat -- TODO: Proper type (enum? Fin?)
+-- TODO: Proper type? Enum ? Fin ?
+abbrev Dir := Nat
+abbrev DirLocal := 0
+abbrev DirWest  := 1
+abbrev DirEast  := 2
+abbrev DirNorth := 3
+abbrev DirSouth := 4
 
 abbrev Flit := Data × FlitHeader
 
@@ -56,7 +62,7 @@ def noc' (name := "noc") : NatModule (NatModule.Named name nocT) :=
 
 -- Implementation --------------------------------------------------------------
 
-def Arbiter := (src : RouterID) → (dest : RouterID) → Option Nat
+def Arbiter := (src : RouterID) → (dest : RouterID) → Option Dir
 
 def routerT := List Flit
 
@@ -88,15 +94,15 @@ def arbiterXY : Arbiter := λ src dst =>
   let dst_x := getX dst
   let dst_y := getY dst
   if src_x == dst_x && src_y == dst_y then
-    .some 0 -- Local output
+    .some DirLocal
   else if src_x < dst_x then
-    .some 1 -- West
+    .some DirWest
   else if dst_x < src_x then
-    .some 2 -- East
+    .some DirEast
   else if src_y < dst_y then
-    .some 3 -- North
+    .some DirNorth
   else if dst_y < src_y then
-    .some 4 -- South
+    .some DirSouth
   else
     .none
 
@@ -104,79 +110,127 @@ def routerXY := router arbiterXY
 
 def ε_noc : Env :=
   [
-    (s!"Router 0", ⟨_, router arbiterXY 0⟩),
-    (s!"Router 1", ⟨_, router arbiterXY 1⟩),
-    (s!"Router 2", ⟨_, router arbiterXY 2⟩),
-    (s!"Router 3", ⟨_, router arbiterXY 3⟩),
+    (s!"Sink Flit", ⟨_, StringModule.sink Flit⟩), -- Sink for unused i/o
+    (s!"Router 0",  ⟨_, router arbiterXY 0⟩),     -- Top left router
+    (s!"Router 1",  ⟨_, router arbiterXY 1⟩),     -- Top right router
+    (s!"Router 2",  ⟨_, router arbiterXY 2⟩),     -- Bot left router
+    (s!"Router 3",  ⟨_, router arbiterXY 3⟩),     -- Bot right router
   ].toAssocList
 
 @[drunfold_defs]
 def noc_low : ExprLow String :=
-  let internal (rID : RouterID) :=
-    InstIdent.internal s!"Router {rID}"
-  let internal_out (rId : RouterID) (dir : Nat) : InternalPort String :=
-    { inst := internal rId, name := NatModule.stringify_output dir }
-  let internal_inp (rId : RouterID) (dir : Nat) : InternalPort String :=
-    { inst := internal rId, name := NatModule.stringify_input dir }
-  let router (rId : RouterID) : ExprLow String := ExprLow.base
+
+  let router_internal (rId : RouterID) :=
+    InstIdent.internal s!"Router {rId}"
+
+  let router_internal_out (rId : RouterID) (dir : Dir) : InternalPort String :=
+    { inst := router_internal rId, name := NatModule.stringify_output dir }
+
+  let router_internal_inp (rId : RouterID) (dir : Dir) : InternalPort String :=
+    { inst := router_internal rId, name := NatModule.stringify_input dir }
+
+  let mkrouter (rId : RouterID) : ExprLow String := ExprLow.base
     {
-      -- 0 is a special case since it is a local port
+      -- 0 is a special case : The local port
       input :=
-        ⟨NatModule.stringify_input 0, NatModule.stringify_input rId⟩ ::
+        ⟨NatModule.stringify_input DirLocal, NatModule.stringify_input rId⟩ ::
         List.map
-          (λ n => ⟨NatModule.stringify_input (n + 1), (internal_inp rId) (n + 1)⟩)
+          (λ n => ⟨NatModule.stringify_input (n + 1), (router_internal_inp rId) (n + 1)⟩)
           (List.range 4)
         |>.toAssocList,
       output :=
-        ⟨NatModule.stringify_output 0, NatModule.stringify_output rId⟩ ::
+        ⟨NatModule.stringify_output DirLocal, NatModule.stringify_output rId⟩ ::
         List.map
-          (λ n => ⟨NatModule.stringify_output (n + 1), (internal_out rId) (n + 1)⟩)
+          (λ n => ⟨NatModule.stringify_output (n + 1), (router_internal_out rId) (n + 1)⟩)
           (List.range 4)
         |>.toAssocList,
     }
     s!"Router {rId}"
-  let base :=
-    router 0 |>
-    ExprLow.product (router 1) |>
-    ExprLow.product (router 2) |>
-    ExprLow.product (router 3)
-  let mkconnection_bi (a b : RouterID) (portA portB : Nat) (base : ExprLow String) :=
+
+  let sink_internal (sId : Nat) :=
+    InstIdent.internal s!"Sink {sId}"
+
+  let sink_internal_inp (sId : Nat) :=
+    { inst := sink_internal sId, name := NatModule.stringify_input 0 }
+
+  -- We use sinks to discard unconnected ports of our routers
+  let mksink (sId : Nat) : ExprLow String := ExprLow.base
+    {
+      input := [⟨NatModule.stringify_input 0, sink_internal_inp sId⟩].toAssocList,
+      output := .nil,
+    }
+    s!"Sink Flit"
+
+  -- Make a bidirectional connection between two routers
+  let mkconn_bi (a b : RouterID) (portA portB : Nat) (base : ExprLow String) :=
     ExprLow.connect
-      { output := internal_out a portA, input := internal_inp b portB } base
+      { output := router_internal_out a portA, input := router_internal_inp b portB } base
     |>
     ExprLow.connect
-      { output := internal_out b portB, input := internal_inp a portA }
+      { output := router_internal_out b portB, input := router_internal_inp a portA }
 
-  let mkconnection_we (w e : RouterID) (base : ExprLow String) :=
-    mkconnection_bi w e 1 2 base
-  let mkconnection_ns (n s : RouterID) (base : ExprLow String) :=
-    mkconnection_bi n s 3 4 base
-  base
-  |> mkconnection_we 0 1
-  |> mkconnection_we 2 3
-  |> mkconnection_ns 0 2
-  |> mkconnection_ns 1 3
+  -- West - East connection
+  let mkconn_we (w e : RouterID) (base : ExprLow String) :=
+    mkconn_bi w e 1 2 base
+
+  -- North -- South connection
+  let mkconn_ns (n s : RouterID) (base : ExprLow String) :=
+    mkconn_bi n s 3 4 base
+
+  -- Connect an output of a router to a sink
+  let mkconn_sink (rId : RouterID) (sId : Nat) (dir : Dir) (base : ExprLow String) :=
+    ExprLow.connect
+      { output := router_internal_out rId dir, input := sink_internal_inp sId }
+      base
+
+  mkrouter 0                    |>  -- Top left router
+  ExprLow.product (mkrouter 1)  |>  -- Top right router
+  ExprLow.product (mkrouter 2)  |>  -- Bot left router
+  ExprLow.product (mkrouter 3)  |>  -- Bot right router
+  ExprLow.product (mksink 0)    |>  -- 0 North
+  ExprLow.product (mksink 1)    |>  -- 0 West
+  ExprLow.product (mksink 2)    |>  -- 1 North
+  ExprLow.product (mksink 3)    |>  -- 1 East
+  ExprLow.product (mksink 4)    |>  -- 2 South
+  ExprLow.product (mksink 5)    |>  -- 2 West
+  ExprLow.product (mksink 6)    |>  -- 3 South
+  ExprLow.product (mksink 7)    |>  -- 3 East
+  mkconn_we 0 1                 |>
+  mkconn_we 2 3                 |>
+  mkconn_ns 0 2                 |>
+  mkconn_ns 1 3                 |>
+  mkconn_sink 0 0 DirNorth      |>
+  mkconn_sink 0 1 DirWest       |>
+  mkconn_sink 1 2 DirNorth      |>
+  mkconn_sink 1 3 DirEast       |>
+  mkconn_sink 2 4 DirSouth      |>
+  mkconn_sink 2 5 DirWest       |>
+  mkconn_sink 3 6 DirSouth      |>
+  mkconn_sink 3 7 DirEast
 
 def noc_lowT : Type := by
   precomputeTac [T| noc_low, ε_noc] by
-    dsimp [drcomponents, ε_noc]
+    dsimp [noc_low, ε_noc]
     dsimp [ExprLow.build_module_type, ExprLow.build_module, ExprLow.build_module']
     simp (disch := simpa) only [toString, drcompute]
 
-@[simp] theorem router_in_env_0 :
+@[simp] theorem sink_in_ε :
+  AssocList.find? "Sink Flit" ε_noc = .some ⟨_, StringModule.sink Flit⟩ := rfl
+
+@[simp] theorem router_in_ε_0 :
   AssocList.find? "Router 0" ε_noc = .some ⟨_, router arbiterXY 0⟩ := rfl
 
-@[simp] theorem router_in_env_1 :
+@[simp] theorem router_in_ε_1 :
   AssocList.find? "Router 1" ε_noc = .some ⟨_, router arbiterXY 1⟩ := rfl
 
-@[simp] theorem router_in_env_2 :
+@[simp] theorem router_in_ε_2 :
   AssocList.find? "Router 2" ε_noc = .some ⟨_, router arbiterXY 2⟩ := rfl
 
-@[simp] theorem router_in_env_3 :
+@[simp] theorem router_in_ε_3 :
   AssocList.find? "Router 3" ε_noc = .some ⟨_, router arbiterXY 3⟩ := rfl
 
 @[drcompute]
-axiom  bijectivePortRenaming_invert' {α} [DecidableEq α] {p : AssocList α α} {i : α}:
+axiom bijectivePortRenaming_invert' {α} [DecidableEq α] {p : AssocList α α} {i : α}:
   p.bijectivePortRenaming i = ((p.filterId.append p.inverse.filterId).find? i).getD i
 
 attribute [-drcompute] AssocList.bijectivePortRenaming_invert
